Updated definitions of random keyed functions to match original model for keyed hash functions and update SPR bounds proof accordingly.

HashFunctionBoundsO.ec
@@ -166,6 +166,13 @@ clone import FinType as FinKey with
 
 clone import FinType as FinIn with
   type t <= input.
+
+clone import FinProdType as FinKeyIn with
+  type t1 <= key,
+  type t2 <- input,
+  
+  theory FT1 <= FinKey,
+  theory FT2 <= FinIn.
   
 clone import FinType as FinOut with
   type t <= output.
@@ -185,6 +192,11 @@ clone import MUniFinFun as MUFF_In with
   
   theory FinT <= FinIn.
 
+clone import MUniFinFun as MUFF_KeyIn with
+  type t <= key * input,
+  
+  theory FinT <= FinKeyIn.
+
 clone import MFinite as MF_Out with
   type t <= output,
   
@@ -193,12 +205,12 @@ clone import MFinite as MF_Out with
 op doutput = MF_Out.dunifin.
 
 clone import BooleanFunctions as BF with
-  type in_t <- input,
+  type in_t <- key * input,
   type out_t <- output,
   
-  theory FinIn <- FinIn,
+  theory FinIn <- FinKeyIn,
   theory FinOut <- FinOut,
-  theory LR.MUFF <- MUFF_In,
+  theory LR.MUFF <- MUFF_KeyIn,
   theory LR.MFY <- MF_Out
   
   proof *.
@@ -210,6 +222,7 @@ op [lossless full uniform] df : (key -> input -> output) distr.
 lemma df_funi : is_funiform df.
 proof. by rewrite is_full_funiform 1:df_fu df_uni. qed.
 
+(*
 op df' : (key -> input -> output) distr =
   dfun (fun (k : key) => dfun (fun (x : input) => doutput)).
 
@@ -234,7 +247,7 @@ proof.
 rewrite dfun_projE /= eq_sym -{1}(dscalar1 (dfun (fun (_ : input) => doutput))) -/df'.
 by congr; rewrite df'_ll is_losslessP 1:dfun_ll //= dunifin_ll.
 qed.
-
+*)
 
 (* Plan:
    - Instantiate KHFO SPR with df
@@ -267,33 +280,33 @@ clone import SPR as KHFO_SPR with
 
 
 module (R_BFFind_SPR (A : Adv_SPR) : Adv_BFFind) (BFO : BFOF_t) = {
-  var f : input -> output
+  var f : key * input -> output
+  var k0 : key
   var x0 : input
   var y0 : output
   
   module O_R_BFFind_SPR : Oracle_t = {
-    proc get(x : input) : output = {
+    proc get(k : key, x : input) : output = {
       var b;
 
-      b <@ BFO.query(x);
+      b <@ BFO.query((k, x));
       
-      return if !b /\ x <> x0 then f x else y0;
+      return if !b /\ (k, x) <> (k0, x0) then f (k, x) else y0;
     }
   }
 
-  proc find() : input = {
-    var k : key;
+  proc find() : key * input = {
     var x' : input;
     
     x0 <$ dinput;
     y0 <$ doutput;
 
-    f <$ MUFF_In.dfun (fun _ => doutput \ (pred1 y0));
+    f <$ MUFF_KeyIn.dfun (fun _ => doutput \ (pred1 y0));
     
-    k <$ dkey;
-    x'  <@ A(O_R_BFFind_SPR).find(k, x0);
+    k0 <$ dkey;
+    x'  <@ A(O_R_BFFind_SPR).find(k0, x0);
     
-    return x';
+    return (k0, x');
   }
 }.
 
@@ -301,6 +314,45 @@ module (R_BFFind_SPR (A : Adv_SPR) : Adv_BFFind) (BFO : BFOF_t) = {
 section.
 
 declare module A <: Adv_SPR {-KHFO.O_Default, -R_BFFind_SPR, -BFOF, -BFOD}.
+
+local op df'_prod : (key * input -> output) distr =
+  dfun (fun (kx : key * input) => doutput).
+
+local lemma df'_prod_ll : is_lossless df'_prod.
+proof. by rewrite &(dfun_ll) /= dunifin_ll. qed.
+
+local lemma df'_prod_fu : is_full df'_prod.
+proof. by rewrite &(dfun_fu) /= dunifin_fu. qed.
+
+local lemma df'_prod_uni : is_uniform df'_prod.
+proof. by rewrite &(dfun_uni) /= dunifin_uni. qed.
+
+local op df' : (key -> input -> output) distr =
+  dmap df'_prod (fun (f : key * input -> output) => 
+                  (fun (k : key) => fun (x : input) => f (k, x))).
+                  
+local lemma df'_ll : is_lossless df'.
+proof. by rewrite &(dmap_ll) /= df'_prod_ll. qed.
+
+local lemma df'_fu : is_full df'.
+proof. 
+rewrite &(dmap_fu) /= 2:df'_prod_fu /surjective.
+move=> f; exists (fun (kx : key * input) => f kx.`1 kx.`2).
+by rewrite fun_ext => k; rewrite fun_ext => x.
+qed.
+
+local lemma df'_uni : is_uniform df'.
+proof.
+rewrite &(dmap_uni) /= 2:df'_prod_uni /injective.
+by move=> f g eqfg; rewrite fun_ext => kx /#.
+qed.
+
+local lemma df'_funi : is_funiform df'.
+proof. by rewrite is_full_funiform 1:df'_fu df'_uni. qed.
+
+local lemma eq_df_df' : df = df'.
+proof. by rewrite &(eq_funi_ll) 1:df_funi 1:df_ll 1:df'_funi df'_ll. qed.
+
 
 local clone import KeyedHashFunctionsO as KHFO' with
   type key_t <- key,
@@ -325,19 +377,19 @@ local equiv Equiv_KHFO_SPR_KHFO'_SPR :
    KHFO_SPR.SPR(A, KHFO.O_Default).main ~ KHFO'_SPR.SPR(A, KHFO'.O_Default).main : ={glob A} ==> ={res}.
 proof.
 proc; inline *.
-call (: ={f, k}(KHFO.O_Default, KHFO'.O_Default)); 1: by proc.
+call (: ={f}(KHFO.O_Default, KHFO'.O_Default)); 1: by proc.
 rnd; wp; rnd; rnd; skip => />.
 by rewrite eq_df_df'.
 qed.
 
-
+(*
 local clone import DMapSampling as DMS with
   type t1 <- key -> input -> output,
   type t2 <- input -> output
   
   proof *.
 
-        
+
 local module O_Default_NK : Oracle_t = {
   var f : input -> output
   
@@ -345,7 +397,7 @@ local module O_Default_NK : Oracle_t = {
     f <- f_init;
   }
   
-  proc get(x : input) : output = {
+  proc get(k : key, x : input) : output = {
     return f x;
   }
 }.
@@ -458,22 +510,152 @@ transitivity SPR_DMS.main
 + by apply Equiv_KHFO'_SPR_SPR_DMS_Main.                
 by apply Equiv_SPR_DMS_Main_SPR_NK.
 qed.
+*)
 
-local module R_Find_SPR_NK_Rand = {
+
+local clone import DMapSampling as DMS with
+  type t1 <- key -> input -> output,
+  type t2 <- key * input -> output
+  
+  proof *.
+
+local module O_Default_Uncurry : Oracle_t = {
+  var f : key * input -> output
+  
+  proc init(f_init : key * input -> output) = {
+    f <- f_init;
+  }
+  
+  proc get(k : key, x : input) : output = {
+    return f (k, x);
+  }
+}.
+
+local module SPR_DMS = {
+  proc main() : bool = {
+    var f : key -> input -> output;
+    var k : key;
+    var x : input;
+    var x' : input;
+
+    f <$ df';
+    k <$ dkey;
+    O_Default_Uncurry.init((fun (kx : key * input) => f kx.`1 kx.`2));
+    x <$ dinput;
+    x' <@ A(O_Default_Uncurry).find(k, x);
+    
+    return x <> x' /\ f k x = f k x';
+  }
+
+  proc main_sample() : bool = {
+    var f : key * input -> output;
+    var k : key;
+    var x : input;
+    var x' : input;
+
+    f <@ S.sample(df', fun f => (fun (kx : key * input) => f kx.`1 kx.`2));
+    k <$ dkey;
+    O_Default_Uncurry.init(f);
+    x <$ dinput;
+    x' <@ A(O_Default_Uncurry).find(k, x);
+
+    return x <> x' /\ f (k, x) = f (k, x');
+  }
+
+  proc main_map() : bool = {
+    var f : key * input -> output;
+    var k : key;
+    var x : input;
+    var x' : input;
+
+    f <@ S.map(df', fun f => (fun (kx : key * input) => f kx.`1 kx.`2));
+    k <$ dkey;
+    O_Default_Uncurry.init(f);
+    x <$ dinput;
+    x' <@ A(O_Default_Uncurry).find(k, x);
+    
+    return x <> x' /\ f (k, x) = f (k, x');
+  }
+}.
+
+local equiv Equiv_KHFO'_SPR_SPR_DMS_Main :
+  KHFO'_SPR.SPR(A, O_Default).main ~ SPR_DMS.main : ={glob A} ==> ={res}. 
+proof.
+proc; inline *.
+call (: forall (k : key) (x : input),
+          O_Default.f{1} k x = O_Default_Uncurry.f{2} (k, x)).
+by proc; skip => /> /#.
+by rnd; wp; rnd; rnd; skip.
+qed.
+
+local module SPR_Uncurry = {
+  proc main() : bool = {
+    var f : key * input -> output;
+    var x, x' : input;
+    var k : key;
+    
+    f <$ df'_prod;
+    k <$ dkey;
+    O_Default_Uncurry.init(f);
+    x <$ dinput;
+    x' <@ A(O_Default_Uncurry).find(k, x);
+
+    return x <> x' /\ f (k, x) = f (k, x');
+  }
+}.
+
+local equiv Equiv_SPR_DMS_Main_SPR_Uncurry :
+  SPR_DMS.main ~ SPR_Uncurry.main : ={glob A} ==> ={res}. 
+proof.
+transitivity SPR_DMS.main_map (={glob A} ==> ={res}) (={glob A} ==> ={res}) => [/# | // | |].
++ proc; inline *.
+  call (: ={O_Default_Uncurry.f}); 1: by proc.
+  swap{1} 2 -1; swap{2} 5 -4.
+  by rnd; wp; rnd; wp; rnd; skip.
+transitivity SPR_DMS.main_sample (={glob A} ==> ={res}) (={glob A} ==> ={res}) => [/# | // | |].
++ proc; inline O_Default_Uncurry.init.
+  call (: ={O_Default_Uncurry.f}); 1: by proc.
+  rnd; wp; rnd => /=.
+  by symmetry; call DMS.sample.
+proc; inline *.
+call (: ={O_Default_Uncurry.f}); 1: by proc.
+rnd; wp; rnd; wp; rnd; wp; skip => />. 
+split => [fR fRin | _ fL] /=; 2: by rewrite df'_prod_fu.
+by rewrite dmap_comp dmap1E /(\o) /pred1; congr; rewrite fun_ext => f /#.
+qed.
+
+local lemma EqPr_SPR_SPR_Uncurry &m :
+  Pr[KHFO_SPR.SPR(A, KHFO.O_Default).main() @ &m : res]
+  =
+  Pr[SPR_Uncurry.main() @ &m : res].
+proof.
+byequiv=> //=.
+transitivity KHFO'_SPR.SPR(A, KHFO'.O_Default).main 
+             (={glob A} ==> ={res}) 
+             (={glob A} ==> ={res}) => [/# | // | |].
++ by apply Equiv_KHFO_SPR_KHFO'_SPR.                
+transitivity SPR_DMS.main 
+             (={glob A} ==> ={res}) 
+             (={glob A} ==> ={res}) => [/# | // | |].
++ by apply Equiv_KHFO'_SPR_SPR_DMS_Main.                
+by apply Equiv_SPR_DMS_Main_SPR_Uncurry.
+qed.
+
+
+local module R_Find_SPR_Uncurry_Rand = {
   import var R_BFFind_SPR
   
-  module O_R_Find_SPR_NK_Rand : Oracle_t = {
-    proc get(x : input) : output = {
+  module O_R_Find_SPR_Uncurry_Rand : Oracle_t = {
+    proc get(k : key, x : input) : output = {
       var b;
 
-      b <@ BFOF.query(x);
+      b <@ BFOF.query((k, x));
       
-      return if !b /\ x <> x0 then f x else y0;
+      return if !b /\ (k, x) <> (k0, x0) then f (k, x) else y0;
     }
   }
 
   proc find() : bool = {
-    var k : key;
     var x' : input;
     var y' : output;
     
@@ -482,19 +664,19 @@ local module R_Find_SPR_NK_Rand = {
     x0 <$ dinput;
     y0 <$ doutput;
 
-    f <$ MUFF_In.dfun (fun _ => doutput \ (pred1 y0));
+    f <$ MUFF_KeyIn.dfun (fun _ => doutput \ (pred1 y0));
     
-    k <$ dkey;
-    x'  <@ A(O_R_Find_SPR_NK_Rand).find(k, x0);
+    k0 <$ dkey;
+    x'  <@ A(O_R_Find_SPR_Uncurry_Rand).find(k0, x0);
     
-    y' <@ O_R_Find_SPR_NK_Rand.get(x');
+    y' <@ O_R_Find_SPR_Uncurry_Rand.get((k0, x'));
     
     return x' <> x0 /\ y' = y0;
   }
 }.
 
-local lemma Find_SPR_NK_Rand_Implies_BFFind &m :
-  Pr[R_Find_SPR_NK_Rand.find() @ &m : res] 
+local lemma Find_SPR_Uncurry_Rand_Implies_BFFind &m :
+  Pr[R_Find_SPR_Uncurry_Rand.find() @ &m : res] 
   <= 
   Pr[BF_Find(R_BFFind_SPR(A), BFOF).main() @ &m : res].
 proof.
@@ -503,64 +685,70 @@ proc; inline *.
 wp.
 conseq (_: ={glob A} 
            ==> 
-               ={BFOF.f, x'} 
-            /\ R_BFFind_SPR.f{1} x'{1} <> R_BFFind_SPR.y0{1}) => />; 1: by smt().
+               ={BFOF.f, R_BFFind_SPR.k0, x'} 
+            /\ R_BFFind_SPR.f{1} (R_BFFind_SPR.k0, x'){1} <> R_BFFind_SPR.y0{1}) => />; 1: by smt().
 call (: ={glob BFOF, glob R_BFFind_SPR}); 1: by sim.
 do 5! rnd; skip => /> fL fLin x0L x0Lin y0L y0Lin fL' + k kin r. 
-by rewrite dfun_supp => /(_ r) /=; rewrite supp_dexcepted /pred1 /= => -[_ ->].
+by rewrite dfun_supp => /(_ (k, r)) /=; rewrite supp_dexcepted /pred1 /= => -[_ ->].
 qed.
 
-local lemma EqPr_SPR_NK_BFFind &m :
-  Pr[SPR_NK.main() @ &m: res] = Pr[R_Find_SPR_NK_Rand.find() @ &m : res].
+local lemma EqPr_SPR_Uncurry_BFFind &m :
+  Pr[SPR_Uncurry.main() @ &m: res] 
+  = 
+  Pr[R_Find_SPR_Uncurry_Rand.find() @ &m : res].
 proof.
 byequiv=> //=.
 proc; inline *.
 wp.
-swap{1} 4 -3; swap{2} 2 -1 => /=.
-seq 1 1: (={glob A} /\ x{1} = R_BFFind_SPR.x0{2}); 1: by rnd.
-call (: forall (x : input), 
-          O_Default_NK.f{1} x 
+swap{1} 2 3.
+swap{1} 4 -3; swap{1} 5 -3.
+swap{2} 2 -1; swap{2} 5 -3 => /=.
+seq 2 2: (   ={glob A} 
+          /\ x{1} = R_BFFind_SPR.x0{2}
+          /\ k{1} = R_BFFind_SPR.k0{2}); 1: by rnd; rnd.
+call (: forall (k : key) (x : input),
+          O_Default_Uncurry.f{1} (k, x) 
           = 
-          if !BFOF.f{2} x /\ x <> R_BFFind_SPR.x0{2} 
-          then R_BFFind_SPR.f{2} x 
+          if !BFOF.f{2} (k, x) /\ (k, x) <> (R_BFFind_SPR.k0, R_BFFind_SPR.x0){2} 
+          then R_BFFind_SPR.f{2} (k, x)
           else R_BFFind_SPR.y0{2}).
 + proc; inline *.
-  by wp; skip => /> &1 &2 /(_ x{2}).
-rnd; wp => />; 1: smt().
-conseq (: _ ==> (forall (x : input), 
-                   f{1} x 
+  by wp; skip => /> &1 &2 /(_ k{2} x{2}).
+wp => />; 1: smt().
+conseq (: _ ==> (forall (k : key) (x : input), 
+                   f{1} (k, x) 
                    = 
-                   if !BFOF.f{2} x /\ x <> R_BFFind_SPR.x0{2} 
-                   then R_BFFind_SPR.f{2} x 
+                   if !BFOF.f{2} (k, x) /\ (k, x) <> (R_BFFind_SPR.k0, R_BFFind_SPR.x0){2}
+                   then R_BFFind_SPR.f{2} (k, x) 
                    else R_BFFind_SPR.y0{2})).
-+ move=> /> &2 fL fR y0 fB ih k kin r.
++ move=> /> &2 fL fR y0 fB ih r.
   by rewrite (eq_sym r); congr; rewrite !ih /= /#.
 transitivity {1} {f <@ LR.LambdaRepro.left();}
   (true ==> ={f}) 
-  (x{1} = R_BFFind_SPR.x0{2} 
+  (k{1} = R_BFFind_SPR.k0{2} /\ x{1} = R_BFFind_SPR.x0{2} 
    ==> 
-   forall (x : input), 
-     f{1} x 
+   forall (k : key) (x : input), 
+     f{1} (k, x) 
      = 
-     if ! BFOF.f{2} x /\ x <>  R_BFFind_SPR.x0{2} 
-     then  R_BFFind_SPR.f{2} x 
+     if ! BFOF.f{2} (k, x) /\ (k, x) <> (R_BFFind_SPR.k0, R_BFFind_SPR.x0){2} 
+     then  R_BFFind_SPR.f{2} (k, x) 
      else  R_BFFind_SPR.y0{2}) => //.
-+ by move=> &1 &2 ?; exists R_BFFind_SPR.x0{2}.
++ by move=> &1 &2 ?; exists R_BFFind_SPR.k0{2} R_BFFind_SPR.x0{2}.
 + by inline *; wp; rnd.
-transitivity {1} {R_BFFind_SPR.f <@ LR.LambdaRepro.right(x);}
+transitivity {1} {R_BFFind_SPR.f <@ LR.LambdaRepro.right(k, x);}
   (true ==> f{1} = R_BFFind_SPR.f{2}) 
-  (x{1} = R_BFFind_SPR.x0{2} 
+  (k{1} = R_BFFind_SPR.k0{2} /\ x{1} = R_BFFind_SPR.x0{2} 
    ==> 
-   forall (x : input), 
-     R_BFFind_SPR.f{1} x 
+   forall (k : key) (x : input), 
+     R_BFFind_SPR.f{1} (k, x) 
      = 
-     if ! BFOF.f{2} x /\ x <> R_BFFind_SPR.x0{2} 
-     then R_BFFind_SPR.f{2} x 
+     if ! BFOF.f{2} (k, x) /\ (k, x) <> (R_BFFind_SPR.k0, R_BFFind_SPR.x0){2} 
+     then R_BFFind_SPR.f{2} (k, x) 
      else R_BFFind_SPR.y0{2}) => //.
-+ by move=> &1 &2 ?; exists R_BFFind_SPR.x0{2}.
++ by move=> &1 &2 ?; exists R_BFFind_SPR.k0{2} R_BFFind_SPR.x0{2}.
 + by call LR.main_theorem. 
-inline *; swap{1} 3 -2.
-by wp; rnd; rnd; wp; rnd; skip.
+inline *; swap{1} 3 -1.
+by wp; rnd; rnd; rnd; wp; skip. 
 qed.
 
 lemma SPR_Implies_BFDistinguish &m:
@@ -571,7 +759,7 @@ lemma SPR_Implies_BFDistinguish &m:
 proof.
 apply (StdOrder.RealOrder.ler_trans Pr[BF_Find(R_BFFind_SPR(A), BFOF).main() @ &m : res]); last first.
 + by rewrite (Find_Implies_Distinguish &m (R_BFFind_SPR(A))).
-by rewrite EqPr_SPR_SPR_NK EqPr_SPR_NK_BFFind Find_SPR_NK_Rand_Implies_BFFind.
+by rewrite EqPr_SPR_SPR_Uncurry EqPr_SPR_Uncurry_BFFind Find_SPR_Uncurry_Rand_Implies_BFFind.
 qed.
 
 end section.
